optimise away constant inps

compiler/RTLOptimizerScript.sml
@@ -6,59 +6,141 @@ open dep_rewrite wordsLib;
 open sumExtraTheory verilogTheory verilogTypeTheory verilogMetaTheory;
 open RTLTheory RTLTypeTheory RTLPropsTheory;
 
-open RTLLib;
+open comparisonTheory balanced_mapTheory;
+
+(*open RTLLib;*)
 
 val _ = new_theory "RTLOptimizer";
-(*
-val cell_not_inp_def = Define `
- (cell_not_inp (Cell1 CNot _ inp) = SOME inp) /\
- (cell_not_inp _ = NONE)`;
 
-val mux_not_cond_opt_def = Define `
- (mux_not_cond_opt above (CellMux out cond tin fin) =
-  case cell_input_num cond of
-    NONE => NONE
-  | SOME n =>
-    case get_cell above n of
-      NONE => NONE
-    | SOME ccond =>
-      case cell_not_inp ccond of
-        NONE => NONE
-      | SOME ccond_inp => SOME (CellMux out ccond_inp fin tin)) /\
- (mux_not_cond_opt above _ = NONE)`
+Datatype:
+ opt_inp = OptConst bool
+         | OptNet num
+End
 
-val THE_default_def = Define `
- (THE_default (SOME x) d = x) /\
- (THE_default NONE d = d)`;
+val _ = type_abbrev_pp ("optm_t", ``:(num, cell_input) balanced_map``);
 
-val muxes_not_cond_opt_def = Define `
- (muxes_not_cond_opt above [] = []) /\
- (muxes_not_cond_opt above (c::cs) =
-  (THE_default (mux_not_cond_opt above c) c) :: muxes_not_cond_opt (c::above) cs)`;
+(*Definition var_cmp_def:
+ (var_cmp (RegVar reg1 n1) (RegVar reg2 n2) =
+  let scmp = string_cmp reg1 reg2 in
+   if scmp = Equal then
+    num_cmp n1 n2
+   else
+    scmp) /\
+ (var_cmp (RegVar _ _) (NetVar _) = Less) /\
+ (var_cmp (NetVar n1) (NetVar n2) = num_cmp n1 n2) /\
+ (var_cmp (NetVar _) (RegVar _ _) = Greater)
+End
 
-(*
-cell_run env h = INR fx ==>
-cell_run env (THE_default (mux_not_cond_opt [] h) h) = INR fx
-
-Theorem muxes_not_cond_opt_correct_lem:
- !cells env env'.
- sum_foldM cell_run env cells = INR env' ==>
- sum_foldM cell_run env (muxes_not_cond_opt [] cells) = INR env'
+Theorem var_cmp_good:
+ good_cmp var_cmp
 Proof
- Induct \\ rw [sum_foldM_def, muxes_not_cond_opt_def, sum_bind_INR] \\
- Cases_on `h` \\ simp [mux_not_cond_opt_def, THE_default_def]
+ rewrite_tac [good_cmp_def] \\ rpt conj_tac \\ rpt Cases \\
+ rw [var_cmp_def] \\ metis_tac [good_cmp_def, string_cmp_good, num_cmp_good, string_cmp_antisym]
 QED
 
-Theorem muxes_not_cond_opt_correct:
- !n cenv cenv' cells regs.
- netlist_run cenv cells regs n = INR cenv' ==>
- netlist_run cenv (muxes_not_cond_opt [] cells) regs n = INR cenv'
+Theorem var_cmp_antisym:
+ !x y. var_cmp x y = Equal <=> x = y
 Proof
- Induct \\ rw [netlist_run_def, sum_bind_INR] \\
- drule_first \\ asm_exists_tac \\
+ Cases \\ Cases \\ rw [var_cmp_def]
+QED*)
 
- fs [netlist_step_def, sum_bind_INR]
-QED
-*)
-*)
+Definition gol_cell_def:
+ (gol_cell (Cell1 _ _ _) = T) ∧
+ (gol_cell (Cell2 t _ _ _) =
+  case t of
+  | CAnd => T
+  | COr => T
+  | CXOr => T
+  | _ => F) ∧
+ (gol_cell _ = F)
+End
+
+Definition opt_cell_input_def:
+ (opt_cell_input m (VarInp (NetVar n) idx) =
+  case lookup num_cmp n m of
+    NONE => VarInp (NetVar n) idx
+  | SOME inp => inp) ∧
+ (opt_cell_input m inp = inp)
+End
+
+Definition bool_of_cell_input_def:
+ (bool_of_cell_input (ConstInp (CBool b)) = SOME b) ∧
+ (bool_of_cell_input _ = NONE)
+End
+
+Definition opt_cell2_1_def:
+ opt_cell2_1 m cell2 out b inp =
+  case cell2 of
+  | CAnd =>
+    if b then
+     (insert num_cmp out inp m, NONE)
+    else
+     (insert num_cmp out (ConstInp (CBool F)) m, NONE)
+  | COr =>
+    if b then
+     (insert num_cmp out (ConstInp (CBool T)) m, NONE)
+    else
+     (insert num_cmp out inp m, NONE)
+  | CXOr =>
+    if b then
+     (m, SOME $ Cell1 CNot out inp)
+    else
+     (insert num_cmp out inp m, NONE)
+  | _ => (m, SOME $ Cell2 cell2 out (ConstInp (CBool b)) inp)
+End
+
+Definition opt_cell2_2_def:
+ opt_cell2_2 cell2 b1 b2 =
+  case cell2 of
+  | CAnd => b1 ∧ b2
+  | COr => b1 ∨ b2
+  | CXOr => b1 ≠ b2
+End
+
+Definition opt_cell_def:
+ (opt_cell m (Cell1 CNot out inp1) =
+  let inp1 = opt_cell_input m inp1 in
+   case bool_of_cell_input inp1 of
+   | NONE => (m, SOME $ Cell1 CNot out inp1)
+   | SOME b => (insert num_cmp out (ConstInp $ CBool ~b) m, NONE)) ∧
+ (opt_cell m (Cell2 cell2 out inp1 inp2) =
+  let inp1 = opt_cell_input m inp1;
+      inp2 = opt_cell_input m inp2 in
+   case (bool_of_cell_input inp1, bool_of_cell_input inp2) of
+   | (NONE, NONE) => (m, SOME $ Cell2 cell2 out inp1 inp2)
+   | (SOME b, NONE) => opt_cell2_1 m cell2 out b inp2
+   | (NONE, SOME b) => opt_cell2_1 m cell2 out b inp1
+   | (SOME b1, SOME b2) => (insert num_cmp out (ConstInp $ CBool $ opt_cell2_2 cell2 b1 b2) m, NONE)) ∧
+ (opt_cell m cell = (m, SOME cell))
+End
+
+Definition opt_netlist_def:
+ (opt_netlist m [] = (m, [])) /\
+ (opt_netlist m (c::cs) =
+  let (m', c') = opt_cell m c;
+      (m'', cs') = opt_netlist m' cs in
+  (m'', case c' of | NONE => cs' | SOME c' => c' :: cs'))
+End
+
+Definition opt_reg_def:
+ opt_reg m (regi, data) =
+  (regi, case data.inp of
+         | NONE => data
+         | SOME inp => data with inp := SOME $ opt_cell_input m inp)
+End
+
+Definition opt_outs_def:
+ (opt_outs m (out, OutInp inp) = (out, OutInp (opt_cell_input m inp))) ∧
+ (opt_outs m (out, OutInps inps) = (out, OutInps (MAP (opt_cell_input m) inps)))
+End
+
+Definition opt_circuit_def:
+ opt_circuit (Circuit extenv outs regs nl_combs nl_ffs) =
+  if EVERY gol_cell nl_combs ∧ ALL_DISTINCT (FLAT $ MAP cell_output nl_combs) then let (* <-- should really be established by blasting, but shortcut for now *)
+   (m, nl_combs) = opt_netlist empty nl_combs in
+   INR $ Circuit extenv (MAP (opt_outs m) outs) (MAP (opt_reg m) regs) nl_combs nl_ffs
+  else
+   INL NotImplemented
+End
+
 val _ = export_theory ();
