compiler/RTLOptimizerProofScript.sml
@@ -1,0 +1,471 @@
+open hardwarePreamble;
+
+open alistTheory wordsTheory;
+open dep_rewrite wordsLib;
+
+open sumExtraTheory verilogTheory verilogTypeTheory verilogMetaTheory;
+open RTLTheory RTLTypeTheory RTLPropsTheory;
+
+open comparisonTheory balanced_mapTheory;
+
+open RTLBlasterProofTheory; (* <-- move blasted_circuit *)
+
+open RTLOptimizerTheory;
+
+val _ = new_theory "RTLOptimizerProof";
+
+infix THEN2;
+infix THEN3;
+
+Definition opt_rel_regs_def:
+ opt_rel_regs (m:optm_t) s opts ⇔
+  opts.fbits = s.fbits ∧
+  (∀n v. cget_var opts (NetVar n) = INR v ⇒ cget_var s (NetVar n) = INR v) ∧
+  (∀reg i. cget_var opts (RegVar reg i) = cget_var s (RegVar reg i)) ∧
+  (∀n. cget_var s (NetVar n) = INL UnknownVariable ⇒ cget_var opts (NetVar n) = INL UnknownVariable) ∧
+  invariant num_cmp m ∧
+  (∀n. case lookup num_cmp n m of
+       | NONE => cget_var opts (NetVar n) = cget_var s (NetVar n)
+       | _ => T)
+End
+
+Definition opt_rel_def:
+ opt_rel fext (m:optm_t) s opts ⇔
+  opt_rel_regs m s opts ∧
+  (∀n. case lookup num_cmp n m of
+       | NONE => cget_var opts (NetVar n) = cget_var s (NetVar n)
+       | SOME inp => ∃b. cget_var s (NetVar n) = INR (CBool b) ∧ cell_inp_run fext opts inp = INR (CBool b))
+End
+
+Definition outs_not_in_env_def:
+ outs_not_in_env nl s ⇔ ∀out. MEM out (FLAT $ MAP cell_output nl) ⇒ cget_var s (NetVar out) = INL UnknownVariable
+End
+
+Triviality only_regs_outs_not_in_env:
+ ∀s nl. only_regs s ⇒ outs_not_in_env nl s
+Proof
+ rw [only_regs_def, outs_not_in_env_def]
+QED
+
+(*
+Actually, cannot prove this because we don't have enough type-information here,
+e.g. Cell1's might be array not... could abort if see such cell with constant input,
+but let's ignore for now and wait for better netlist representation with static types.
+
+Definition is_ConstInp_def:
+ (is_ConstInp (ConstInp _) = T) ∧
+ (is_ConstInp (ExtInp _ _) = F) ∧
+ (is_ConstInp (VarInp _ _) = F)
+End
+
+(* only relevant for gol cells *)
+Definition cell_has_no_ConstInp_def:
+ (cell_has_no_ConstInp (Cell1 t out inp1) ⇔ ~is_ConstInp inp1) ∧
+ (cell_has_no_ConstInp (Cell2 t out inp1 inp2) ⇔ ~is_ConstInp inp2 ∧ ~is_ConstInp inp1) ∧
+ (* overapproximate the rest *)
+ (cell_has_no_ConstInp _ ⇔ T)
+End
+
+(* only checks cells! *)
+Definition circuit_has_no_ConstInp_def:
+ circuit_has_no_ConstInp (Circuit _ _ _ nl1 nl2) ⇔
+ EVERY cell_has_no_ConstInp nl1 ∧ EVERY cell_has_no_ConstInp nl2
+End
+*)
+
+Triviality opt_rel_regs_sym:
+ ∀s. opt_rel_regs empty s s
+Proof
+ simp [opt_rel_regs_def, invariant_def, empty_def] \\ gen_tac \\ CASE_TAC
+QED
+
+Triviality opt_rel_opt_rel_regs:
+ ∀fext s opts. opt_rel fext empty s opts ⇔ opt_rel_regs empty s opts
+Proof
+ rw [opt_rel_regs_def, opt_rel_def] \\ eq_tac \\ rw [empty_def, lookup_def, invariant_def]
+QED
+
+Triviality opt_rel_regs_cset_var:
+ opt_rel_regs m s1 s2 ⇒
+ opt_rel_regs m (cset_var s1 (RegVar reg i) v) (cset_var s2 (RegVar reg i) v)
+Proof
+ rw [opt_rel_regs_def, cget_var_cset_var]
+QED
+
+Triviality opt_rel_cset_var:
+ ∀fext m s1 s2 n v.
+ opt_rel fext m s1 s2 ∧
+ cget_var s1 (NetVar n) = INL UnknownVariable ⇒
+ opt_rel fext m (cset_var s1 (NetVar n) v) (cset_var s2 (NetVar n) v)
+Proof
+ rw [opt_rel_def]
+ >- (fs [opt_rel_regs_def, cget_var_cset_var] \\ rw [] \\ CASE_TAC)
+ >- (CASE_TAC \\ rw [cget_var_cset_var]
+     >- (last_x_assum (qspec_then ‘n'’ assume_tac) \\ gs [])
+     >- (last_x_assum (qspec_then ‘n’ assume_tac) \\ gs [])
+     >- (last_x_assum (qspec_then ‘n'’ assume_tac) \\ gs [] \\
+         fs [opt_rel_regs_def] \\ drule_first \\
+         rename1 ‘cell_inp_run _ _ inp’ \\ Cases_on ‘inp’ \\
+         fs [cell_inp_run_def, cget_var_cset_var] \\
+         rw [] \\ fs [sum_bind_def]))
+QED
+
+val lookup_insert_num_cmp =
+ MATCH_MP (CONV_RULE (REWR_CONV (GSYM AND_IMP_INTRO)) lookup_insert) num_cmp_good
+ |> REWRITE_RULE [num_cmp_antisym];
+
+val insert_thm_num_cmp =
+ MATCH_MP (CONV_RULE (REWR_CONV (GSYM AND_IMP_INTRO)) (SPEC_ALL insert_thm)) num_cmp_good;
+
+Triviality opt_rel_cset_var_insert_inp:
+ ∀inp fext m s1 s2 n b.
+ opt_rel fext m s1 s2 ∧
+ cell_inp_run fext s2 inp = INR (CBool b) ∧
+ cget_var s1 (NetVar n) = INL UnknownVariable ⇒
+ opt_rel fext (insert num_cmp n inp m) (cset_var s1 (NetVar n) (CBool b)) s2
+Proof
+ rw [opt_rel_def, opt_rel_regs_def]
+ THEN3 (fs [cget_var_cset_var] \\ every_case_tac \\ gvs [])
+ >- simp [insert_thm_num_cmp]
+ THEN2 (rw [lookup_insert_num_cmp] \\ simp [cget_var_cset_var, cell_inp_run_def])
+QED
+
+Triviality opt_rel_cset_var_insert:
+ ∀fext m s1 s2 n b.
+ opt_rel fext m s1 s2 ∧
+ cget_var s1 (NetVar n) = INL UnknownVariable ⇒
+ opt_rel fext (insert num_cmp n (ConstInp (CBool b)) m) (cset_var s1 (NetVar n) (CBool b)) s2
+Proof
+ metis_tac [opt_rel_cset_var_insert_inp, cell_inp_run_def]
+QED
+
+Triviality opt_cell_input_correct:
+ ∀inp m s1 s2 v fext.
+ cell_inp_run fext s1 inp = INR v ∧
+ opt_rel fext m s1 s2 ⇒
+ cell_inp_run fext s2 (opt_cell_input m inp) = INR v
+Proof
+ Cases \\ simp [opt_cell_input_def] THEN2 (simp [cell_inp_run_def]) \\ rpt strip_tac \\
+ rename1 ‘VarInp var idx’ \\ Cases_on ‘var’ \\ fs [opt_cell_input_def, opt_rel_def]
+ >- fs [opt_rel_regs_def, cell_inp_run_def] \\
+ last_x_assum (qspec_then ‘n’ assume_tac) \\ CASE_TAC \\
+ gvs [cell_inp_run_def, sum_bind_INR] \\
+ Cases_on ‘idx’ \\ fs [cget_fext_var_def]
+QED
+
+Triviality sum_mapM_opt_cell_input_correct:
+ ∀inps m s1 s2 v fext.
+ sum_mapM (cell_inp_run fext s1) inps = INR v ∧
+ opt_rel fext m s1 s2 ⇒
+ sum_mapM (cell_inp_run fext s2) (MAP (opt_cell_input m) inps) = INR v
+Proof
+ Induct \\ simp [sum_mapM_INR] \\ metis_tac [opt_cell_input_correct]
+QED
+
+Triviality bool_of_cell_input_correct:
+ ∀inp fext s v b.
+ bool_of_cell_input inp = SOME b ∧ cell_inp_run fext s inp = INR v ⇒
+ v = CBool b
+Proof
+ Cases \\ TRY (Cases_on ‘v’) \\ rw [cell_inp_run_def, bool_of_cell_input_def]
+QED
+
+Triviality opt_cell2_1_correct:
+ ∀t inp1 inp2 b v v' fext s sopt m m' cellopt out.
+ opt_cell2_1 m t out b inp2 = (m', cellopt) ∧
+ cell2_run t (CBool b) v' = INR v ∧
+ cell_inp_run fext sopt inp1 = INR (CBool b) ∧
+ cell_inp_run fext sopt inp2 = INR v' ∧
+ gol_cell (Cell2 t out inp1 inp2) ∧
+ opt_rel fext m s sopt ∧
+ cget_var s (NetVar out) = INL UnknownVariable ⇒
+ (case cellopt of
+ | NONE => opt_rel fext m' (cset_var s (NetVar out) v) sopt
+ | SOME cellopt => ∃sopt'. cell_run fext sopt cellopt = INR sopt' ∧
+                           opt_rel fext m' (cset_var s (NetVar out) v) sopt') ∧
+ OPTION_ALL gol_cell cellopt
+Proof
+ Cases \\ rw [opt_cell2_1_def, gol_cell_def] \\
+ Cases_on ‘v'’ \\ gvs [cell2_run_def] \\
+ TRY (match_mp_tac opt_rel_cset_var_insert_inp \\ simp [cell_inp_run_def]) \\
+ simp [cell_run_def, cell1_run_def, sum_bind_def, gol_cell_def] \\
+ match_mp_tac opt_rel_cset_var \\ simp []
+QED
+
+Triviality cell2_run_comm:
+ ∀t v1 v2. cell2_run t v1 v2 = cell2_run t v2 v1
+Proof
+ rpt Cases \\ rw [cell2_run_def] \\ simp [EQ_SYM_EQ] \\
+ rw [sum_check_def, sum_bind_def] \\ metis_tac []
+QED
+
+Triviality gol_cell_Cell2_new_inps:
+ ∀t. gol_cell (Cell2 t out inp1 inp2) ⇔ gol_cell (Cell2 t out inp1' inp2')
+Proof
+ Cases \\ rw [gol_cell_def]
+QED
+
+Triviality opt_circuit_run_cell:
+ ∀cell cellopt m m' s1 s1' s2 fext.
+ opt_cell m cell = (m', cellopt) ∧
+ cell_run fext s1 cell = INR s1' ∧
+ opt_rel fext m s1 s2 ∧
+ (∀out. MEM out (cell_output cell) ⇒ cget_var s1 (NetVar out) = INL UnknownVariable) ∧
+ gol_cell cell ⇒
+ (case cellopt of
+  | NONE => opt_rel fext m' s1' s2
+  | SOME cellopt => ∃s2'. cell_run fext s2 cellopt = INR s2' ∧
+                          opt_rel fext m' s1' s2') ∧
+ OPTION_ALL gol_cell cellopt
+Proof
+ Cases \\ TRY (simp [gol_cell_def] \\ NO_TAC) \\ rpt strip_tac'
+
+ (* Cell1 *)
+ >- (rename1 ‘Cell1 t _ _’ \\ Cases_on ‘t’ \\
+     fs [cell_output_def, cell_run_def, cell1_run_def, sum_bind_INR, opt_cell_def] \\
+
+     drule_strip opt_cell_input_correct \\
+
+     every_case_tac \\ gvs [] \\ simp [cell_run_def, gol_cell_def]
+     >- (drule_strip bool_of_cell_input_correct \\
+         gvs [cell1_run_def] \\
+         match_mp_tac opt_rel_cset_var_insert \\ simp [])
+     >- (simp [sum_bind_def] \\
+         match_mp_tac opt_rel_cset_var \\ simp []))
+
+ (* Cell2 *)
+ >- (rename1 ‘Cell2 t out inp1 inp2’ \\
+     fs [cell_output_def, cell_run_def, cell2_run_def, sum_bind_INR, opt_cell_def] \\
+     qspec_then ‘inp1’ assume_tac opt_cell_input_correct \\ drule_first \\
+     qspec_then ‘inp2’ assume_tac opt_cell_input_correct \\ drule_first \\
+
+     last_x_assum mp_tac \\ CASE_TAC \\ CASE_TAC \\ strip_tac
+
+     >- (rveq \\ fs [cell_run_def, sum_bind_def] \\ conj_tac
+         >- (match_mp_tac opt_rel_cset_var \\ simp [])
+         >- (Cases_on ‘t’ \\ fs [gol_cell_def]))
+     >- (drule_strip bool_of_cell_input_correct \\
+         drule_strip opt_cell2_1_correct \\ metis_tac [gol_cell_Cell2_new_inps])
+     >- (fs [Once cell2_run_comm] \\
+         drule_strip bool_of_cell_input_correct \\
+         drule_strip opt_cell2_1_correct \\ metis_tac [gol_cell_Cell2_new_inps])
+     >- (rveq \\
+         imp_res_tac bool_of_cell_input_correct \\ gvs [] \\
+         Cases_on ‘t’ \\ fs [gol_cell_def] \\ Cases_on ‘x’ \\ Cases_on ‘x'’ \\
+         fs [cell2_run_def] \\
+         match_mp_tac opt_rel_cset_var_insert_inp \\
+         simp [cell_inp_run_def, opt_cell2_2_def]))
+QED
+
+Triviality opt_circuit_run_cells:
+ ∀nl1 nl1' m m' s1 s1' s2 fext.
+ opt_netlist m nl1 = (m', nl1') ∧
+ sum_foldM (cell_run fext) s1 nl1 = INR s1' ∧
+ opt_rel fext m s1 s2 ∧
+ outs_not_in_env nl1 s1 ∧
+ ALL_DISTINCT (FLAT $ MAP cell_output nl1) ∧
+ EVERY gol_cell nl1 ⇒
+ ∃s2'. sum_foldM (cell_run fext) s2 nl1' = INR s2' ∧
+       opt_rel fext m' s1' s2' ∧
+       EVERY gol_cell nl1'
+Proof
+ Induct \\ simp [opt_netlist_def, sum_foldM_INR] \\ rpt strip_tac' \\
+ fs [outs_not_in_env_def] \\ fs [ALL_DISTINCT_APPEND] \\
+
+ pairarg_tac \\ fs [] \\
+ drule_strip opt_circuit_run_cell \\ impl_tac >- simp [] \\ strip_tac \\
+ pairarg_tac \\ fs [] \\ rveq \\
+
+ CASE_TAC \\ fs [] \\
+ drule_first \\ (impl_tac >- metis_tac [cell_run_unchanged]) \\ simp [sum_foldM_INR]
+QED
+
+Triviality opt_reg_correct:
+ ∀regs fext snet1 snet2 sreg1 sreg1' sreg2 m.
+ sum_foldM (reg_run fext snet1) sreg1 regs = INR sreg1' ∧
+ opt_rel fext m snet1 snet2 ∧
+ opt_rel_regs empty sreg1 sreg2 ⇒
+ ∃sreg2'. sum_foldM (reg_run fext snet2) sreg2 (MAP (opt_reg m) regs) = INR sreg2' ∧
+          opt_rel_regs empty sreg1' sreg2'
+Proof
+ Induct >- simp [sum_foldM_def] \\ Cases \\ rename1 ‘(regi, _)’ \\ Cases_on ‘regi’ \\
+ simp [sum_foldM_INR, reg_run_def] \\ rpt gen_tac \\
+ CASE_TAC >- (rpt strip_tac \\ drule_first \\ simp [opt_reg_def, reg_run_def]) \\
+ rpt strip_tac \\ fs [sum_bind_INR] \\ rveq \\
+ drule_strip opt_cell_input_correct \\
+ simp [opt_reg_def, reg_run_def, sum_bind_def] \\
+ qmatch_goalsub_abbrev_tac ‘sum_foldM _ sreg2' _’ \\
+ drule_first \\ disch_then (qspec_then ‘sreg2'’ mp_tac) \\
+ unabbrev_all_tac \\ impl_tac >- (match_mp_tac opt_rel_regs_cset_var \\ simp []) \\
+ strip_tac \\ simp []
+QED
+
+Triviality cget_var_FILTER_is_RegVar_NetVar:
+ ∀s n. cget_var (s with env := FILTER (is_RegVar ∘ FST) s.env) (NetVar n) = INL UnknownVariable
+Proof
+ rw [cget_var_def, ALOOKUP_FILTER_FST, is_RegVar_def]
+QED
+
+Triviality cget_var_FILTER_is_RegVar_RegVar:
+ ∀s reg i.
+ cget_var (s with env := FILTER (is_RegVar ∘ FST) s.env) (RegVar reg i) = cget_var s (RegVar reg i)
+Proof
+ rw [cget_var_def, ALOOKUP_FILTER_FST, is_RegVar_def]
+QED
+
+Triviality opt_circuit_netlist_run_no_pseudos:
+ ∀n nl1 nl1' m fext s1 s1' s2 regs.
+ opt_netlist empty nl1 = (m, nl1') ∧
+ netlist_run_no_pseudos fext s1 nl1 regs n = INR s1' ∧
+ opt_rel_regs empty s1 s2 ∧
+ outs_not_in_env nl1 s1 ∧
+ ALL_DISTINCT (FLAT $ MAP cell_output nl1) ∧
+ EVERY gol_cell nl1 ⇒
+ ∃s2'. netlist_run_no_pseudos fext s2 nl1' (MAP (opt_reg m) regs) n = INR s2' ∧
+       opt_rel (fext n) m s1' s2' ∧
+       EVERY gol_cell nl1'
+Proof
+ Induct
+ >- (rpt strip_tac' \\
+     fs [netlist_run_no_pseudos_def] \\
+     drule_strip opt_circuit_run_cells \\
+     simp [opt_rel_opt_rel_regs])
+
+ >- (rpt strip_tac' \\
+     fs [netlist_run_no_pseudos_def, sum_bind_INR] \\
+     drule_first \\
+     simp [] \\
+     qmatch_goalsub_abbrev_tac ‘sum_foldM _ s2'reg _’ \\
+     drule_strip opt_reg_correct \\
+     disch_then (qspec_then ‘s2'reg’ mp_tac) \\
+     unabbrev_all_tac \\
+     impl_tac >- (fs [opt_rel_def, opt_rel_regs_def,
+                      cget_var_FILTER_is_RegVar_NetVar, cget_var_FILTER_is_RegVar_RegVar] \\
+                  simp [lookup_def, empty_def]) \\ strip_tac \\
+     simp [] \\
+     drule_strip opt_circuit_run_cells \\
+     disch_then (qspec_then ‘sreg2'’ mp_tac) \\
+     impl_tac >- (metis_tac [opt_rel_opt_rel_regs, regs_run_only_regs,
+                             only_regs_FILTER_is_RegVar, only_regs_outs_not_in_env]) \\ strip_tac \\
+     simp [])
+QED
+
+Triviality opt_circuit_init_run:
+ ∀regs m s s'.
+ init_run s regs = INR s' ⇒ init_run s (MAP (opt_reg m) regs) = INR s'
+Proof
+ Induct >- rw [init_run_def] \\ Cases \\ rename1 ‘(regi, _)’ \\ Cases_on ‘regi’ \\ rw [opt_reg_def, init_run_def] \\
+ every_case_tac \\ gs [] \\ pairarg_tac \\ fs []
+QED
+
+Triviality opt_outs_correct:
+ ∀outs s1 s2 s' fext m.
+ sum_mapM (out_run fext s1) outs = INR s' ∧
+ opt_rel fext m s1 s2 ⇒
+ sum_mapM (out_run fext s2) (MAP (opt_outs m) outs) = INR s'
+Proof
+ Induct >- simp [sum_mapM_def] \\ Cases \\ rename1 ‘(out, spec)’ \\ simp [sum_mapM_INR] \\ rpt strip_tac \\
+ rveq \\ Cases_on ‘spec’
+ >- (fs [opt_outs_def, out_run_def, sum_bind_INR] \\
+     drule_strip opt_cell_input_correct \\
+     simp [] \\ drule_first)
+ >- (fs [opt_outs_def, out_run_def, sum_bind_INR] \\
+     drule_strip sum_mapM_opt_cell_input_correct \\
+     simp [] \\ drule_first)
+QED
+
+Triviality opt_circuit_regs_type_and_nl_ffs_lem:
+ ∀cir cir'.
+ opt_circuit cir = INR cir' ⇒
+ EVERY (λ(_,rdata). rdata.reg_type = Reg) (circuit_regs cir') =
+ EVERY (λ(_,rdata). rdata.reg_type = Reg) (circuit_regs cir) ∧
+ circuit_nl_ffs cir' = circuit_nl_ffs cir
+Proof
+ Cases \\ simp [opt_circuit_def] \\ rpt strip_tac' \\ every_case_tac \\ fs [] \\ pairarg_tac \\ fs [] \\ rveq \\
+ simp [circuit_regs_def, circuit_nl_ffs_def, EVERY_MAP] \\ match_mp_tac EVERY_CONG \\ simp [] \\
+ Cases \\ rw [opt_reg_def] \\ every_case_tac \\ simp []
+QED
+
+Triviality EVERY_gol_cell_deterministic_netlist:
+ ∀nl. EVERY gol_cell nl ⇒ deterministic_netlist nl
+Proof
+ rw [deterministic_netlist_def, EVERY_MEM] \\ drule_first \\
+ Cases_on ‘e’ \\ fs [gol_cell_def, deterministic_cell_def]
+QED
+
+Triviality FST_opt_reg:
+ FST ∘ (opt_reg m) = FST
+Proof
+ simp [FUN_EQ_THM] \\ Cases \\ simp [opt_reg_def]
+QED
+
+Triviality blast_regs_distinct_opt_reg:
+ ∀regs m. blast_regs_distinct (MAP (opt_reg m) regs) = blast_regs_distinct regs
+Proof
+ rw [blast_regs_distinct_def, MAP_MAP_o, blast_reg_name_def, FST_opt_reg]
+QED
+
+Triviality reg_reg_type_opt_reg_lem:
+ EVERY (λ(_,rdata). rdata.reg_type = Reg) (MAP (opt_reg m) regs) =
+ EVERY (λ(_,rdata). rdata.reg_type = Reg) regs
+Proof
+ rw [EVERY_MAP] \\ match_mp_tac EVERY_CONG \\ simp [] \\ PairCases \\ rw [opt_reg_def] \\
+ CASE_TAC \\ rw []
+QED
+
+Triviality reg_type_opt_reg_lem:
+ EVERY (λ(_,rdata). rdata.type = CBool_t) (MAP (opt_reg m) regs) =
+ EVERY (λ(_,rdata). rdata.type = CBool_t) regs
+Proof
+ rw [EVERY_MAP] \\ match_mp_tac EVERY_CONG \\ simp [] \\ PairCases \\ rw [opt_reg_def] \\
+ CASE_TAC \\ rw []
+QED
+
+Triviality deterministic_regs_opt_reg_lem:
+ deterministic_regs (MAP (opt_reg m) regs) = deterministic_regs regs
+Proof
+ rw [deterministic_regs_def, EVERY_MAP] \\ match_mp_tac EVERY_CONG \\ simp [] \\ PairCases \\ rw [opt_reg_def] \\
+ CASE_TAC \\ rw [deterministic_reg_def]
+QED
+
+Theorem opt_circuit_correct:
+ ∀cir cir' fext fbits n s.
+ opt_circuit cir = INR cir' ∧
+ blasted_circuit cir ∧
+ circuit_run fext fbits cir n = INR s ⇒
+ blasted_circuit cir' ∧
+ circuit_run fext fbits cir' n = INR s
+Proof
+ Cases \\ simp [blasted_circuit_def] \\ rpt strip_tac' \\ first_x_assum mp_tac \\
+ DEP_REWRITE_TAC [circuit_run_circuit_run_no_pseudos] \\
+ conj_tac >- (drule_strip opt_circuit_regs_type_and_nl_ffs_lem \\
+              fs [circuit_regs_def, circuit_nl_ffs_def]) \\ strip_tac \\
+
+ fs [opt_circuit_def] \\ every_case_tac \\ fs [] \\ pairarg_tac \\ fs [] \\ rveq \\
+ fs [circuit_run_no_pseudos_def, sum_bind_INR] \\ rveq \\
+
+ drule_strip opt_circuit_init_run \\ simp [] \\
+ drule_strip opt_circuit_netlist_run_no_pseudos \\
+ disch_then (qspec_then ‘s'’ mp_tac) \\
+ impl_tac >- (drule_strip init_run_only_regs \\ simp [only_regs_nil] \\ strip_tac \\
+              simp [only_regs_outs_not_in_env, opt_rel_regs_sym]) \\ strip_tac \\
+ simp [] \\
+ conj_tac >- (drule_strip EVERY_gol_cell_deterministic_netlist \\
+              fs [blasted_circuit_def] \\
+              metis_tac [blast_regs_distinct_opt_reg, reg_reg_type_opt_reg_lem,
+                         reg_type_opt_reg_lem, deterministic_regs_opt_reg_lem]) \\
+ drule_strip opt_outs_correct \\
+ fs [opt_rel_def, opt_rel_regs_def]
+QED
+
+Theorem opt_circuit_const:
+ ∀cir cir' fext.
+ opt_circuit cir = INR cir' ⇒
+ (rtltype_extenv (circuit_extenv cir') fext = rtltype_extenv (circuit_extenv cir) fext) ∧
+ (MAP FST (circuit_regs cir') = MAP FST (circuit_regs cir))
+Proof
+ Cases \\ rw [opt_circuit_def] \\ pairarg_tac \\ fs [] \\ rveq \\
+ simp [circuit_extenv_def, circuit_regs_def, MAP_MAP_o, FST_opt_reg]
+QED
+
+val _ = export_theory ();
